backend/SelectDivproof.v
@@ -1,0 +1,547 @@
+(* *********************************************************************)
+(*                                                                     *)
+(*              The Compcert verified compiler                         *)
+(*                                                                     *)
+(*          Xavier Leroy, INRIA Paris-Rocquencourt                     *)
+(*                                                                     *)
+(*  Copyright Institut National de Recherche en Informatique et en     *)
+(*  Automatique.  All rights reserved.  This file is distributed       *)
+(*  under the terms of the INRIA Non-Commercial License Agreement.     *)
+(*                                                                     *)
+(* *********************************************************************)
+
+(** Correctness of instruction selection for integer division *)
+
+Require Import Coqlib.
+Require Import Zquot.
+Require Import AST.
+Require Import Integers.
+Require Import Floats.
+Require Import Values.
+Require Import Memory.
+Require Import Globalenvs.
+Require Import Events.
+Require Import Cminor.
+Require Import Op.
+Require Import CminorSel.
+Require Import SelectOp.
+Require Import SelectOpproof.
+Require Import SelectDiv.
+
+Open Local Scope cminorsel_scope.
+
+(** * Main approximation theorems *)
+
+Section Z_DIV_MUL.
+
+Variable N: Z.      (**r number of relevant bits *)
+Hypothesis N_pos: N >= 0.
+Variable d: Z.      (**r divisor *)
+Hypothesis d_pos: d > 0.
+
+(** This is theorem 4.2 from Granlund and Montgomery, PLDI 1994. *)
+
+Lemma Zdiv_mul_pos:
+  forall m l,
+  l >= 0 ->
+  two_p (N+l) <= m * d <= two_p (N+l) + two_p l ->
+  forall n,
+  0 <= n < two_p N ->
+  Zdiv n d = Zdiv (m * n) (two_p (N + l)).
+Proof.
+  intros m l l_pos [LO HI] n RANGE.
+  exploit (Z_div_mod_eq n d). auto. 
+  set (q := n / d).
+  set (r := n mod d).
+  intro EUCL.
+  assert (0 <= r <= d - 1).
+    unfold r. generalize (Z_mod_lt n d d_pos). omega.
+  assert (0 <= m). 
+    apply Zmult_le_0_reg_r with d. auto.
+    exploit (two_p_gt_ZERO (N + l)). omega. omega. 
+  set (k := m * d - two_p (N + l)).
+  assert (0 <= k <= two_p l). 
+    unfold k; omega.
+  assert ((m * n - two_p (N + l) * q) * d = k * n + two_p (N + l) * r).
+    unfold k. rewrite EUCL. ring.
+  assert (0 <= k * n).
+    apply Zmult_le_0_compat; omega.
+  assert (k * n <= two_p (N + l) - two_p l).
+    apply Zle_trans with (two_p l * n).
+    apply Zmult_le_compat_r. omega. omega.
+    replace (N + l) with (l + N) by omega.
+    rewrite two_p_is_exp. 
+    replace (two_p l * two_p N - two_p l)
+       with (two_p l * (two_p N - 1))
+         by ring.
+    apply Zmult_le_compat_l. omega. exploit (two_p_gt_ZERO l). omega. omega.
+    omega. omega.
+  assert (0 <= two_p (N + l) * r).
+    apply Zmult_le_0_compat. 
+    exploit (two_p_gt_ZERO (N + l)). omega. omega.
+    omega.
+  assert (two_p (N + l) * r <= two_p (N + l) * d - two_p (N + l)).
+    replace (two_p (N + l) * d - two_p (N + l))
+       with (two_p (N + l) * (d - 1)) by ring.
+    apply Zmult_le_compat_l.
+    omega.
+    exploit (two_p_gt_ZERO (N + l)). omega. omega.
+  assert (0 <= m * n - two_p (N + l) * q).
+    apply Zmult_le_reg_r with d. auto. 
+    replace (0 * d) with 0 by ring.  rewrite H2. omega. 
+  assert (m * n - two_p (N + l) * q < two_p (N + l)).
+    apply Zmult_lt_reg_r with d. omega.
+    rewrite H2. 
+    apply Zle_lt_trans with (two_p (N + l) * d - two_p l).
+    omega. 
+    exploit (two_p_gt_ZERO l). omega. omega.
+  symmetry. apply Zdiv_unique with (m * n - two_p (N + l) * q). 
+  ring. omega.
+Qed.
+
+Lemma Zdiv_unique_2:
+  forall x y q, y > 0 -> 0 < y * q - x <= y -> Zdiv x y = q - 1.
+Proof.
+  intros. apply Zdiv_unique with (x - (q - 1) * y). ring. 
+  replace ((q - 1) * y) with (y * q - y) by ring. omega. 
+Qed.
+
+Lemma Zdiv_mul_opp:
+  forall m l,
+  l >= 0 ->
+  two_p (N+l) < m * d <= two_p (N+l) + two_p l ->
+  forall n,
+  0 < n <= two_p N ->
+  Zdiv n d = - Zdiv (m * (-n)) (two_p (N + l)) - 1.
+Proof.
+  intros m l l_pos [LO HI] n RANGE.
+  replace (m * (-n)) with (- (m * n)) by ring.
+  exploit (Z_div_mod_eq n d). auto. 
+  set (q := n / d).
+  set (r := n mod d).
+  intro EUCL.
+  assert (0 <= r <= d - 1).
+    unfold r. generalize (Z_mod_lt n d d_pos). omega.
+  assert (0 <= m). 
+    apply Zmult_le_0_reg_r with d. auto.
+    exploit (two_p_gt_ZERO (N + l)). omega. omega.
+  cut (Zdiv (- (m * n)) (two_p (N + l)) = -q - 1).
+    omega.
+  apply Zdiv_unique_2. 
+  apply two_p_gt_ZERO. omega.
+  replace (two_p (N + l) * - q - - (m * n))
+     with (m * n - two_p (N + l) * q)
+       by ring.
+  set (k := m * d - two_p (N + l)).
+  assert (0 < k <= two_p l). 
+    unfold k; omega.
+  assert ((m * n - two_p (N + l) * q) * d = k * n + two_p (N + l) * r).
+    unfold k. rewrite EUCL. ring.
+  split.
+  apply Zmult_lt_reg_r with d. omega. 
+  replace (0 * d) with 0 by omega.
+  rewrite H2.
+  assert (0 < k * n). apply Zmult_lt_0_compat; omega.
+  assert (0 <= two_p (N + l) * r).
+    apply Zmult_le_0_compat. exploit (two_p_gt_ZERO (N + l)); omega. omega.
+  omega.
+  apply Zmult_le_reg_r with d. omega.
+  rewrite H2. 
+  assert (k * n <= two_p (N + l)).
+    rewrite Zplus_comm. rewrite two_p_is_exp; try omega. 
+    apply Zle_trans with (two_p l * n). apply Zmult_le_compat_r. omega. omega. 
+    apply Zmult_le_compat_l. omega. exploit (two_p_gt_ZERO l). omega. omega.
+  assert (two_p (N + l) * r <= two_p (N + l) * d - two_p (N + l)).
+    replace (two_p (N + l) * d - two_p (N + l))
+       with (two_p (N + l) * (d - 1))
+         by ring.
+    apply Zmult_le_compat_l. omega. exploit (two_p_gt_ZERO (N + l)). omega. omega.
+  omega.
+Qed.
+
+(** This is theorem 5.1 from Granlund and Montgomery, PLDI 1994. *)
+
+Lemma Zquot_mul:
+  forall m l,
+  l >= 0 ->
+  two_p (N+l) < m * d <= two_p (N+l) + two_p l ->
+  forall n,
+  - two_p N <= n < two_p N ->
+  Z.quot n d = Zdiv (m * n) (two_p (N + l)) + (if zlt n 0 then 1 else 0).
+Proof.
+  intros. destruct (zlt n 0).
+  exploit (Zdiv_mul_opp m l H H0 (-n)). omega. 
+  replace (- - n) with n by ring.
+  replace (Z.quot n d) with (- Z.quot (-n) d).
+  rewrite Zquot_Zdiv_pos by omega. omega.
+  rewrite Z.quot_opp_l by omega. ring.
+  rewrite Zplus_0_r. rewrite Zquot_Zdiv_pos by omega. 
+  apply Zdiv_mul_pos; omega.
+Qed.
+
+End Z_DIV_MUL.
+
+(** * Correctness of the division parameters *)
+
+Lemma divs_mul_params_sound:
+  forall d m p,
+  divs_mul_params d = Some(p, m) ->
+  0 <= m < Int.modulus /\ 0 <= p < 32 /\
+  forall n,
+  Int.min_signed <= n <= Int.max_signed ->
+  Z.quot n d = Zdiv (m * n) (two_p (32 + p)) + (if zlt n 0 then 1 else 0).
+Proof with (try discriminate).
+  unfold divs_mul_params; intros d m' p' EQ.
+  destruct (find_div_mul_params Int.wordsize
+               (Int.half_modulus - Int.half_modulus mod d - 1) d 32)
+  as [[p m] | ]...
+  destruct (zlt 0 d)...
+  destruct (zlt (two_p (32 + p)) (m * d))...
+  destruct (zle (m * d) (two_p (32 + p) + two_p (p + 1)))...
+  destruct (zle 0 m)...
+  destruct (zlt m Int.modulus)...
+  destruct (zle 0 p)...
+  destruct (zlt p 32)...
+  simpl in EQ. inv EQ. 
+  split. auto. split. auto. intros. 
+  replace (32 + p') with (31 + (p' + 1)) by omega. 
+  apply Zquot_mul; try omega.
+  replace (31 + (p' + 1)) with (32 + p') by omega. omega.
+  change (Int.min_signed <= n < Int.half_modulus). 
+  unfold Int.max_signed in H. omega. 
+Qed.
+
+Lemma divu_mul_params_sound:
+  forall d m p,
+  divu_mul_params d = Some(p, m) ->
+  0 <= m < Int.modulus /\ 0 <= p < 32 /\
+  forall n,
+  0 <= n < Int.modulus ->
+  Zdiv n d = Zdiv (m * n) (two_p (32 + p)).
+Proof with (try discriminate).
+  unfold divu_mul_params; intros d m' p' EQ.
+  destruct (find_div_mul_params Int.wordsize
+               (Int.modulus - Int.modulus mod d - 1) d 32)
+  as [[p m] | ]...
+  destruct (zlt 0 d)...
+  destruct (zle (two_p (32 + p)) (m * d))...
+  destruct (zle (m * d) (two_p (32 + p) + two_p p))...
+  destruct (zle 0 m)...
+  destruct (zlt m Int.modulus)...
+  destruct (zle 0 p)...
+  destruct (zlt p 32)...
+  simpl in EQ. inv EQ. 
+  split. auto. split. auto. intros.
+  apply Zdiv_mul_pos; try omega. assumption.
+Qed.
+
+Lemma divs_mul_shift_gen:
+  forall x y m p,
+  divs_mul_params (Int.signed y) = Some(p, m) ->
+  0 <= m < Int.modulus /\ 0 <= p < 32 /\
+  Int.divs x y = Int.add (Int.shr (Int.repr ((Int.signed x * m) / Int.modulus)) (Int.repr p))
+                         (Int.shru x (Int.repr 31)).
+Proof.
+  intros. set (n := Int.signed x). set (d := Int.signed y) in *.
+  exploit divs_mul_params_sound; eauto. intros (A & B & C).
+  split. auto. split. auto.
+  unfold Int.divs. fold n; fold d. rewrite C by (apply Int.signed_range). 
+  rewrite two_p_is_exp by omega. rewrite <- Zdiv_Zdiv. 
+  rewrite Int.shru_lt_zero. unfold Int.add. apply Int.eqm_samerepr. apply Int.eqm_add.
+  rewrite Int.shr_div_two_p. apply Int.eqm_unsigned_repr_r. apply Int.eqm_refl2. 
+  rewrite Int.unsigned_repr. f_equal.
+  rewrite Int.signed_repr. rewrite Int.modulus_power. f_equal. ring.
+  cut (Int.min_signed <= n * m / Int.modulus < Int.half_modulus). 
+  unfold Int.max_signed; omega. 
+  apply Zdiv_interval_1. generalize Int.min_signed_neg; omega. apply Int.half_modulus_pos. 
+  apply Int.modulus_pos.
+  split. apply Zle_trans with (Int.min_signed * m). apply Zmult_le_compat_l_neg. omega. generalize Int.min_signed_neg; omega.
+  apply Zmult_le_compat_r. unfold n; generalize (Int.signed_range x); tauto. tauto.
+  apply Zle_lt_trans with (Int.half_modulus * m). 
+  apply Zmult_le_compat_r. generalize (Int.signed_range x); unfold n, Int.max_signed; omega. tauto.
+  apply Zmult_lt_compat_l. generalize Int.half_modulus_pos; omega. tauto. 
+  assert (32 < Int.max_unsigned) by (compute; auto). omega.
+  unfold Int.lt; fold n. rewrite Int.signed_zero. destruct (zlt n 0); apply Int.eqm_unsigned_repr. 
+  apply two_p_gt_ZERO. omega.
+  apply two_p_gt_ZERO. omega.
+Qed.
+
+Theorem divs_mul_shift_1:
+  forall x y m p,
+  divs_mul_params (Int.signed y) = Some(p, m) ->
+  m < Int.half_modulus ->
+  0 <= p < 32 /\
+  Int.divs x y = Int.add (Int.shr (Int.mulhs x (Int.repr m)) (Int.repr p))
+                         (Int.shru x (Int.repr 31)).
+Proof.
+  intros. exploit divs_mul_shift_gen; eauto. instantiate (1 := x). 
+  intros (A & B & C). split. auto. rewrite C. 
+  unfold Int.mulhs. rewrite Int.signed_repr. auto.
+  generalize Int.min_signed_neg; unfold Int.max_signed; omega.
+Qed.
+
+Theorem divs_mul_shift_2:
+  forall x y m p,
+  divs_mul_params (Int.signed y) = Some(p, m) ->
+  m >= Int.half_modulus ->
+  0 <= p < 32 /\
+  Int.divs x y = Int.add (Int.shr (Int.add (Int.mulhs x (Int.repr m)) x) (Int.repr p))
+                         (Int.shru x (Int.repr 31)).
+Proof.
+  intros. exploit divs_mul_shift_gen; eauto. instantiate (1 := x). 
+  intros (A & B & C). split. auto. rewrite C. f_equal. f_equal.
+  rewrite Int.add_signed. unfold Int.mulhs. set (n := Int.signed x).
+  transitivity (Int.repr (n * (m - Int.modulus) / Int.modulus + n)).
+  f_equal. 
+  replace (n * (m - Int.modulus)) with (n * m +  (-n) * Int.modulus) by ring.
+  rewrite Z_div_plus. ring. apply Int.modulus_pos. 
+  apply Int.eqm_samerepr. apply Int.eqm_add; auto with ints. 
+  apply Int.eqm_sym. eapply Int.eqm_trans. apply Int.eqm_signed_unsigned. 
+  apply Int.eqm_unsigned_repr_l. apply Int.eqm_refl2. f_equal. f_equal. 
+  rewrite Int.signed_repr_eq. rewrite Zmod_small by assumption. 
+  apply zlt_false. omega.
+Qed.
+
+Theorem divu_mul_shift:
+  forall x y m p,
+  divu_mul_params (Int.unsigned y) = Some(p, m) ->
+  0 <= p < 32 /\
+  Int.divu x y = Int.shru (Int.mulhu x (Int.repr m)) (Int.repr p).
+Proof.
+  intros. exploit divu_mul_params_sound; eauto. intros (A & B & C).
+  split. auto. 
+  rewrite Int.shru_div_two_p. rewrite Int.unsigned_repr. 
+  unfold Int.divu, Int.mulhu. f_equal. rewrite C by apply Int.unsigned_range.
+  rewrite two_p_is_exp by omega. rewrite <- Zdiv_Zdiv by (apply two_p_gt_ZERO; omega).
+  f_equal. rewrite (Int.unsigned_repr m). 
+  rewrite Int.unsigned_repr. f_equal. ring.
+  cut (0 <= Int.unsigned x * m / Int.modulus < Int.modulus).
+  unfold Int.max_unsigned; omega.
+  apply Zdiv_interval_1. omega. compute; auto. compute; auto.
+  split. simpl. apply Z.mul_nonneg_nonneg. generalize (Int.unsigned_range x); omega. omega. 
+  apply Zle_lt_trans with (Int.modulus * m).
+  apply Zmult_le_compat_r. generalize (Int.unsigned_range x); omega. omega. 
+  apply Zmult_lt_compat_l. compute; auto. omega. 
+  unfold Int.max_unsigned; omega.
+  assert (32 < Int.max_unsigned) by (compute; auto). omega.
+Qed.
+
+(** * Correctness of the smart constructors for division and modulus *)
+
+Section CMCONSTRS.
+
+Variable ge: genv.
+Variable sp: val.
+Variable e: env.
+Variable m: mem.
+
+Lemma eval_divu_mul:
+  forall le x y p M,
+  divu_mul_params (Int.unsigned y) = Some(p, M) ->
+  nth_error le O = Some (Vint x) ->
+  eval_expr ge sp e m le (divu_mul p M) (Vint (Int.divu x y)).
+Proof.
+  intros. unfold divu_mul. exploit (divu_mul_shift x); eauto. intros [A B].
+  assert (eval_expr ge sp e m le
+           (Eop Omulhu (Eletvar 0 ::: Eop (Ointconst (Int.repr M)) Enil ::: Enil))
+           (Vint (Int.mulhu x (Int.repr M)))).
+  { EvalOp. econstructor. econstructor; eauto. econstructor. EvalOp. simpl; reflexivity. constructor.
+    auto. }
+  exploit eval_shruimm. eexact H1. instantiate (1 := Int.repr p). 
+  intros [v [P Q]]. simpl in Q. 
+  replace (Int.ltu (Int.repr p) Int.iwordsize) with true in Q. 
+  inv Q. rewrite B. auto. 
+  unfold Int.ltu. rewrite Int.unsigned_repr. rewrite zlt_true; auto. tauto.
+  assert (32 < Int.max_unsigned) by (compute; auto). omega.
+Qed.
+
+Theorem eval_divuimm:
+  forall le e1 x n2 z,
+  eval_expr ge sp e m le e1 x ->
+  Val.divu x (Vint n2) = Some z ->
+  exists v, eval_expr ge sp e m le (divuimm e1 n2) v /\ Val.lessdef z v.
+Proof.
+  unfold divuimm; intros. generalize H0; intros DIV.
+  destruct x; simpl in DIV; try discriminate.
+  destruct (Int.eq n2 Int.zero) eqn:Z2; inv DIV. 
+  destruct (Int.is_power2 n2) as [l | ] eqn:P2.
+- erewrite Int.divu_pow2 by eauto. 
+  replace (Vint (Int.shru i l)) with (Val.shru (Vint i) (Vint l)). 
+  apply eval_shruimm; auto.
+  simpl. erewrite Int.is_power2_range; eauto. 
+- destruct (divu_mul_params (Int.unsigned n2)) as [[p M] | ] eqn:PARAMS.
+  + exists (Vint (Int.divu i n2)); split; auto.
+    econstructor; eauto. eapply eval_divu_mul; eauto. 
+  + eapply eval_divu_base; eauto. EvalOp.
+Qed.
+
+Theorem eval_divu:
+  forall le a b x y z,
+  eval_expr ge sp e m le a x ->
+  eval_expr ge sp e m le b y ->
+  Val.divu x y = Some z ->
+  exists v, eval_expr ge sp e m le (divu a b) v /\ Val.lessdef z v.
+Proof.
+  unfold divu; intros until b. destruct (divu_match b); intros.
+- inv H0. inv H5. simpl in H7. inv H7. eapply eval_divuimm; eauto.
+- eapply eval_divu_base; eauto. 
+Qed.
+
+Lemma eval_mod_from_div:
+  forall le a n x y,
+  eval_expr ge sp e m le a (Vint y) ->
+  nth_error le O = Some (Vint x) ->
+  eval_expr ge sp e m le (mod_from_div a n) (Vint (Int.sub x (Int.mul y n))).
+Proof.
+  unfold mod_from_div; intros. 
+  exploit eval_mulimm; eauto. instantiate (1 := n). intros [v [A B]]. 
+  simpl in B. inv B. EvalOp.
+Qed.
+
+Theorem eval_moduimm:
+  forall le e1 x n2 z,
+  eval_expr ge sp e m le e1 x ->
+  Val.modu x (Vint n2) = Some z ->
+  exists v, eval_expr ge sp e m le (moduimm e1 n2) v /\ Val.lessdef z v.
+Proof.
+  unfold moduimm; intros. generalize H0; intros MOD.
+  destruct x; simpl in MOD; try discriminate.
+  destruct (Int.eq n2 Int.zero) eqn:Z2; inv MOD. 
+  destruct (Int.is_power2 n2) as [l | ] eqn:P2.
+- erewrite Int.modu_and by eauto.
+  change (Vint (Int.and i (Int.sub n2 Int.one)))
+    with (Val.and (Vint i) (Vint (Int.sub n2 Int.one))).
+  apply eval_andimm. auto.
+- destruct (divu_mul_params (Int.unsigned n2)) as [[p M] | ] eqn:PARAMS.
+  + econstructor; split. 
+    econstructor; eauto. eapply eval_mod_from_div. 
+    eapply eval_divu_mul; eauto. simpl; eauto. simpl; eauto. 
+    rewrite Int.modu_divu. auto. 
+    red; intros; subst n2; discriminate.
+  + eapply eval_modu_base; eauto. EvalOp.
+Qed.
+
+Theorem eval_modu:
+  forall le a b x y z,
+  eval_expr ge sp e m le a x ->
+  eval_expr ge sp e m le b y ->
+  Val.modu x y = Some z ->
+  exists v, eval_expr ge sp e m le (modu a b) v /\ Val.lessdef z v.
+Proof.
+  unfold modu; intros until b. destruct (modu_match b); intros.
+- inv H0. inv H5. simpl in H7. inv H7. eapply eval_moduimm; eauto.
+- eapply eval_modu_base; eauto. 
+Qed.
+
+Lemma eval_divs_mul:
+  forall le x y p M,
+  divs_mul_params (Int.signed y) = Some(p, M) ->
+  nth_error le O = Some (Vint x) ->
+  eval_expr ge sp e m le (divs_mul p M) (Vint (Int.divs x y)).
+Proof.
+  intros. unfold divs_mul.
+  assert (V: eval_expr ge sp e m le (Eletvar O) (Vint x)).
+  { constructor; auto. }
+  assert (X: eval_expr ge sp e m le
+           (Eop Omulhs (Eletvar 0 ::: Eop (Ointconst (Int.repr M)) Enil ::: Enil))
+           (Vint (Int.mulhs x (Int.repr M)))).
+  { EvalOp. econstructor. eauto. econstructor. EvalOp. simpl; reflexivity. constructor.
+    auto. }
+  exploit eval_shruimm. eexact V. instantiate (1 := Int.repr (Int.zwordsize - 1)). 
+  intros [v1 [Y LD]]. simpl in LD. 
+  change (Int.ltu (Int.repr 31) Int.iwordsize) with true in LD. 
+  simpl in LD. inv LD. 
+  assert (RANGE: 0 <= p < 32 -> Int.ltu (Int.repr p) Int.iwordsize = true).
+  { intros. unfold Int.ltu. rewrite Int.unsigned_repr. rewrite zlt_true by tauto. auto.
+    assert (32 < Int.max_unsigned) by (compute; auto). omega. }
+  destruct (zlt M Int.half_modulus).
+- exploit (divs_mul_shift_1 x); eauto. intros [A B].
+  exploit eval_shrimm. eexact X. instantiate (1 := Int.repr p). intros [v1 [Z LD]].
+  simpl in LD. rewrite RANGE in LD by auto. inv LD.
+  exploit eval_add. eexact Z. eexact Y. intros [v1 [W LD]].
+  simpl in LD. inv LD. 
+  rewrite B. exact W.
+- exploit (divs_mul_shift_2 x); eauto. intros [A B].
+  exploit eval_add. eexact X. eexact V. intros [v1 [Z LD]]. 
+  simpl in LD. inv LD. 
+  exploit eval_shrimm. eexact Z. instantiate (1 := Int.repr p). intros [v1 [U LD]].
+  simpl in LD. rewrite RANGE in LD by auto. inv LD.
+  exploit eval_add. eexact U. eexact Y. intros [v1 [W LD]].
+  simpl in LD. inv LD. 
+  rewrite B. exact W.
+Qed.
+
+Theorem eval_divsimm:
+  forall le e1 x n2 z,
+  eval_expr ge sp e m le e1 x ->
+  Val.divs x (Vint n2) = Some z ->
+  exists v, eval_expr ge sp e m le (divsimm e1 n2) v /\ Val.lessdef z v.
+Proof.
+  unfold divsimm; intros. generalize H0; intros DIV.
+  destruct x; simpl in DIV; try discriminate.
+  destruct (Int.eq n2 Int.zero
+            || Int.eq i (Int.repr Int.min_signed) && Int.eq n2 Int.mone) eqn:Z2; inv DIV. 
+  destruct (Int.is_power2 n2) as [l | ] eqn:P2.
+- destruct (Int.ltu l (Int.repr 31)) eqn:LT31.
+  + eapply eval_shrximm; eauto. eapply Val.divs_pow2; eauto.
+  + eapply eval_divs_base; eauto. EvalOp.
+- destruct (divs_mul_params (Int.signed n2)) as [[p M] | ] eqn:PARAMS.
+  + exists (Vint (Int.divs i n2)); split; auto.
+    econstructor; eauto. eapply eval_divs_mul; eauto. 
+  + eapply eval_divs_base; eauto. EvalOp.
+Qed.
+
+Theorem eval_divs:
+  forall le a b x y z,
+  eval_expr ge sp e m le a x ->
+  eval_expr ge sp e m le b y ->
+  Val.divs x y = Some z ->
+  exists v, eval_expr ge sp e m le (divs a b) v /\ Val.lessdef z v.
+Proof.
+  unfold divs; intros until b. destruct (divs_match b); intros.
+- inv H0. inv H5. simpl in H7. inv H7. eapply eval_divsimm; eauto.
+- eapply eval_divs_base; eauto. 
+Qed.
+
+Theorem eval_modsimm:
+  forall le e1 x n2 z,
+  eval_expr ge sp e m le e1 x ->
+  Val.mods x (Vint n2) = Some z ->
+  exists v, eval_expr ge sp e m le (modsimm e1 n2) v /\ Val.lessdef z v.
+Proof.
+  unfold modsimm; intros. 
+  exploit Val.mods_divs; eauto. intros [y [A B]].
+  generalize A; intros DIV.
+  destruct x; simpl in DIV; try discriminate.
+  destruct (Int.eq n2 Int.zero
+            || Int.eq i (Int.repr Int.min_signed) && Int.eq n2 Int.mone) eqn:Z2; inv DIV. 
+  destruct (Int.is_power2 n2) as [l | ] eqn:P2.
+- destruct (Int.ltu l (Int.repr 31)) eqn:LT31.
+  + exploit (eval_shrximm ge sp e m (Vint i :: le) (Eletvar O)).
+    constructor. simpl; eauto. eapply Val.divs_pow2; eauto. 
+    intros [v1 [X LD]]. inv LD. 
+    econstructor; split. econstructor. eauto. 
+    apply eval_mod_from_div. eexact X. simpl; eauto. 
+    simpl. auto.
+  + eapply eval_mods_base; eauto. EvalOp.
+- destruct (divs_mul_params (Int.signed n2)) as [[p M] | ] eqn:PARAMS.
+  + econstructor; split. 
+    econstructor. eauto. apply eval_mod_from_div with (x := i); auto.
+    eapply eval_divs_mul with (x := i); eauto.
+    simpl. auto.
+  + eapply eval_mods_base; eauto. EvalOp.
+Qed.
+
+Theorem eval_mods:
+  forall le a b x y z,
+  eval_expr ge sp e m le a x ->
+  eval_expr ge sp e m le b y ->
+  Val.mods x y = Some z ->
+  exists v, eval_expr ge sp e m le (mods a b) v /\ Val.lessdef z v.
+Proof.
+  unfold mods; intros until b. destruct (mods_match b); intros.
+- inv H0. inv H5. simpl in H7. inv H7. eapply eval_modsimm; eauto.
+- eapply eval_mods_base; eauto. 
+Qed.
+
+End CMCONSTRS.
